
$\displaystyle\sum\limits_{n=1}^{\infty}=lim_{n\to+\infty}(1^2+\frac{1}{2^2}+\frac{1}{3^2}+\cdots+\frac{1}{n^2})$


$sinx = x-\frac{x^3}{3!}+\frac{x^5}{5!}-\frac{x^7}{7!}+\cdots$
$\frac{sinx}{x} = 1-\frac{x^2}{3!}+\frac{x^4}{5!}-\frac{x^6}{7!}+\cdots$



$$
\begin{aligned} \frac{sinx}{x} &= (1-\frac{x}{\pi})\left(1+\frac{x}{\pi}\right)(1+\frac{x}{2\pi})(1-\frac{x}{2\pi})(1+\frac{x}{3\pi})(1-\frac{x}{3\pi})\cdots\\   &=(1-\frac{x^2}{\pi^2})(1-\frac{x^2}{4\pi^2})(1-\frac{x^2}{9\pi^2})\cdots \end{aligned}
$$

$$
-(\frac{1}{\pi^2}+\frac{1}{4\pi^2}+\frac{1}{9\pi^2}+\frac{1}{16\pi^{2}})=-\frac{1}{\pi^2}\displaystyle\sum\limits_{n=1}^{\infty}\frac{1}{n^2}
$$


$$
-\frac16 = -\frac{1}{\pi^2}\displaystyle\sum\limits_{n=1}^{\infty}\frac{1}{n^2}
$$

$$
\displaystyle\sum\limits_{n=1}^{\infty}\frac{1}{n^2}=\frac{\pi^2}{6}
$$


$\begin{bmatrix}3\quad2\quad1\\1\quad2\quad5\end{bmatrix}$
